some backup

SEARNarith.sml
@@ -1,3 +1,7 @@
+val o_assoc = Thm_2_7_assoc
+
+val o_Fun = Thm_2_7_o_Fun
+
 local
 val lemma = 
  fVar_Inst 
@@ -180,7 +184,7 @@ e0
  last_x_assum irule >> first_x_assum accept_tac
  )
 (form_goal
- “!X a:mem(X) f:X->X. isFun(f) ==>
+ “!X a:mem(X) f:X->X. isFun(f) ==> 
  ?u:N->X. isFun(u) & Eval(u,O) = a & 
  !n:mem(N).Eval(u,Eval(SUC,n)) = Eval(f,Eval(u,n))”));
 end
@@ -276,64 +280,157 @@ val Eval_o_eq = Eval_o_eq0 |> strip_all_and_imp |> gen_all
 
 val Eval_eq_o = GSYM Eval_o_eq |> store_as "Eval_eq_o";
 
+local
+val l = 
+(fVar_Inst [("P",([("d",mem_sort ONE),("x",mem_sort $ mk_set ("A"))],
+“d = dot & x = a:mem(A)”))] (AX1 |> qspecl [‘1’,‘A’])) 
+|> uex_expand
+in
+val El_ex = prove_store("El_ex",
+e0
+(rpt strip_tac >> strip_assume_tac l >>
+ qexists_tac ‘R’ >> 
+ qby_tac ‘isFun(R)’ >-- (rw[Fun_expand] >> arw[] >>
+ rpt strip_tac >-- (qexists_tac ‘a’ >> rw[dot_def]) >> arw[]) >>
+ arw[] >> drule $ GSYM Eval_def >> flip_tac >> arw[])
+(form_goal
+ “!A a:mem(A).?el:1->A.isFun(el) & Eval(el,dot) = a”))
+end
 
+
+val El_def = El_ex |> spec_all |> ex2fsym0 "El" ["a"]
+                   |> gen_all
+                   |> store_as "El_def";
+
+
+val Eval_El = prove_store("Eval_El",
+e0
+(rpt strip_tac >>
+ qspecl_then [‘A’,‘a’] strip_assume_tac El_def >> 
+ rw[dot_def] >> arw[]
+ )
+(form_goal
+ “!A a:mem(A) x. Eval(El(a),x) = a”));
+
+val El_Fun = El_def |> spec_all |> conjE1 |> gen_all
+                    |> store_as "El_Fun";
 
 
 val Nind_alt = prove_store("Nind_O",
 e0
-(rpt strip_tac >> uex_tac >> qexists_tac ‘Nind(a,f)’ >> 
- drule Nind_def >> arw[] >>
- rpt strip_tac (* 2 *)
- >-- (irule $ iffRL FUN_EXT >> 
+(rpt strip_tac >--
+ (drule Nind_def >> arw[]) >-- (drule Nind_def >> arw[]) 
+ >-- (drule Nind_def >> irule $ iffRL FUN_EXT >> 
      first_x_assum (qspecl_then [‘a’] strip_assume_tac) >>
      qby_tac ‘isFun(Nind(a,f) o SUC) & isFun(f o Nind(a, f))’
      >-- (strip_tac >> irule o_Fun >> arw[SUC_isFun]) >>
      arw[] >> strip_tac >> irule $ iffRL Eval_eq_o >>
      arw[SUC_Fun])
  (*irule does not work without strip*) >>
+ drule Nind_def >>
  first_x_assum (qspecl_then [‘a’] strip_assume_tac) >>
  first_x_assum irule >> arw[] >> 
  strip_tac >> irule $ iffLR Eval_eq_o >>
  arw[SUC_Fun]
  )
 (form_goal
- “!X a:mem(X) f:X->X. isFun(f) ==>
- ?!u:N->X. isFun(u) & Eval(u,O) = a & 
- u o SUC = f o u”));
+ “!X  f:X->X. isFun(f) ==>
+ !a:mem(X).isFun(Nind(a,f)) & Eval(Nind(a,f),O) = a & 
+ Nind(a,f) o SUC = f o Nind(a,f) &
+ (!u. (isFun(u) & Eval(u,O) = a & u o SUC = f o u) ==> u = Nind(a,f))”));
 
 
-val Thm1_case1_comm_condition_left = prove_store(
-"Thm1_case1_comm_condition_left",
+val is_Nind = Nind_alt |> strip_all_and_imp
+                       |> conjE2
+                       |> conjE2
+                       |> conjE2 |> gen_all
+                       |> disch_all |> gen_all
+                       |> store_as "is_Nind";
+
+val El_eq_eq = prove_store("El_eq_eq",
 e0
-(rpt strip_tac >> rw[Pa_distr,idL] >> dimp_tac >> strip_tac
+(rpt strip_tac >> dimp_tac >> strip_tac 
+ >-- (qby_tac ‘isFun(El(a)) & isFun(El(b))’
+     >-- rw[El_Fun] >> 
+     drule FUN_EXT >> fs[] >> 
+     last_x_assum (qspecl_then [‘dot’] assume_tac) >>
+     fs[El_def]) >> 
+ arw[])
+(form_goal
+ “!A a:mem(A) b. El(a) = El(b) <=> a = b”));
+
+
+
+
+val Eval_o_l = prove_store("Eval_o_l",
+e0
+(rpt strip_tac >>
+ qsuff_tac
+ ‘Eval(g o f, a) = Eval(g, Eval(f, a))’
+ >-- (strip_tac >> arw[])
+  >> irule $ GSYM o_Eval >> arw[])
+(form_goal
+ “!A B f:A->B.isFun(f) ==> !C g:B->C.isFun(g) ==>
+  !a c. Eval(g o f,a) = c <=>
+ Eval(g,Eval(f,a)) = c”));
+
+val Eval_o_El = prove_store("Eval_o_El",
+e0
+(rpt strip_tac >> flip_tac >> irule $ iffRL Eval_o_l >>
+ arw[El_Fun] >> rw[El_def])
+(form_goal
+ “!A B f:A->B.isFun(f) ==>
+  !a. Eval(f,a) = Eval(f o El(a),dot)”));
+
+val Nind_El = prove_store("Nind_el",
+e0
+(strip_tac >> strip_tac >> strip_tac >>
+ drule Nind_def >> strip_tac >>
+ first_x_assum (qspecl_then [‘a’] strip_assume_tac) >>
+ arw[] >> rpt strip_tac (* 3 *)
+ >-- irule $ iffRL FUN_EXT >> rpt strip_tac (* 3 *)
+     >-- (irule $ iffRL Eval_o_l >> arw[Eval_El,El_Fun])
+     >-- (irule o_Fun >> arw[El_Fun] (* arw bug that does not use El_Fun *)
+         >> rw[El_Fun]) >>
+     rw[El_Fun]
+ >-- (irule $ iffRL FUN_EXT >> rpt strip_tac (*3*)
+     >-- (irule $ iffLR Eval_o_eq >> 
+          arw[SUC_Fun]) 
+     >-- (irule o_Fun >> arw[SUC_Fun]) >>
+     irule o_Fun >> arw[]) >>
+ first_x_assum irule >> arw[] >> rpt strip_tac (* 2 *)
+ >-- (irule $ iffRL Eval_o_eq >> arw[] >> rw[SUC_Fun]) >>
+ drule Eval_o_El >> arw[] >> rw[El_def])
+(form_goal
+ “!X  f:X->X. isFun(f) ==>
+ !a:mem(X).isFun(Nind(a,f)) & Nind(a,f) o El(O) = El(a) & 
+ Nind(a,f) o SUC = f o Nind(a,f) &
+ (!u. (isFun(u) & u o El(O) = El(a) & u o SUC = f o u) ==> u = Nind(a,f))”));
+
+
+
+val Eval_El_mem = prove_store("Eval_El_mem",
+e0
+(rpt strip_tac >> dimp_tac >> strip_tac (* 2 *)
+ >-- (irule $iffRL FUN_EXT >> rpt strip_tac (* 3 *)
+     >-- (rw[Eval_El] >> irule $iffRL Eval_o_l >>
+         arw[Eval_El,El_Fun]) 
+     >-- (irule o_Fun >> arw[El_Fun]) >>
+     rw[El_Fun]) >>
+ qby_tac ‘Eval(f o El(a),dot) = Eval(El(b),dot)’ 
  >-- arw[] >>
- fs[Pa_eq_eq])
+ pop_assum mp_tac >> rw[Eval_El] >> strip_tac >>
+ qsuff_tac ‘Eval(f o El(a), dot) = Eval(f,a)’ 
+ >-- (strip_tac >> arw[] >> fs[]) >>
+ irule $ iffRL Eval_o_l >>
+ arw[El_def])
 (form_goal
- “!B f:N->B g:1->B. Eval(Pa(id(N),f),O) = Pa(O,g) <=> Eval(f,O) = Eval(g,dot)”));
- 
-val Thm1_case1_comm_condition_right = prove_store(
-"Thm1_case1_comm_condition_right",
-e0
-(rpt strip_tac >> 
- rw[Pa_distr,o_assoc,p1_of_Pa,idL,idR,Pa_eq_eq])
-(form_goal
- “!B f:N->B h:N * B ->B.
- Pa(SUC o p1(N,B),h) o Pa(id(N),f) = Pa(id(N),f) o SUC <=>
- h o Pa(id(N),f) = f o SUC”));
-
-val Thm1_case1_comm_condition = prove_store(
-"Thm1_case1_comm_condition",
-e0
-(rpt strip_tac >> 
- rw[Thm1_case1_comm_condition_left,
- Thm1_case1_comm_condition_right] >> dimp_tac >> strip_tac >> arw[])
-(form_goal
- “!B f0:N->B g:1->B h:N * B -> B. f0 o O = g & f0 o SUC = h o Pa(id(N),f0) <=>
- Pa(id(N),f0) o O = Pa(O,g) &
- Pa(SUC o p1(N,B),h) o Pa(id(N),f0) = Pa(id(N),f0) o SUC”));
+ “!A B f:A->B. isFun(f) ==> !a b. Eval(f,a) = b <=>
+ f o El(a) = El(b)”));
 
 
-val comm_with_SUC_id = prove_store("comm_with_SUC_id",
+
+val comm_with_SUC_id0 = prove_store("comm_with_SUC_id0",
 e0
 (qspecl_then [‘N’,‘SUC’] strip_assume_tac Nind_def >>
  assume_tac SUC_isFun >> first_x_assum drule >>
@@ -351,34 +448,292 @@ e0
  rw[Eval_id,id_Fun]
  )
 (form_goal
- “!f:N->N. isFun(f) ==>Eval(f,O) = O & f o SUC = SUC o f ==> f = id(N)”));
+ “!f:N->N. isFun(f) ==> Eval(f,O) = O & f o SUC = SUC o f ==> f = id(N)”));
 
-val is_Nind = Nind_def |> spec_all |> undisch |> conjE2
-                       |> disch_all |> gen_all
-                       |> store_as "is_Nind";
 
-val o_assoc = Thm_2_7_assoc
+val comm_with_SUC_id = prove_store("comm_with_SUC_id",
+e0
+(strip_tac >> strip_tac >> 
+ drule comm_with_SUC_id0 >> drule Eval_El_mem >>
+ fs[])
+(form_goal
+ “!f:N->N. isFun(f) ==> f o El(O) = El(O) & f o SUC = SUC o f ==> f = id(N)”));
 
-val o_Fun = Thm_2_7_o_Fun
+
+val Pa_distr = prove_store("Pa_distr",
+e0
+(rpt strip_tac >> irule is_Pa >> 
+ qspecl_then [‘A’,‘X’,‘a1’,‘B’,‘a2’] strip_assume_tac pi12_of_Pa >>
+ rfs[] >> rw[GSYM o_assoc] >> arw[] >> 
+ qspecl_then [‘A’,‘X’,‘a1’,‘B’,‘a2’] strip_assume_tac Pa_Fun >>
+ rfs[] >> rpt strip_tac >>
+ irule o_Fun >> arw[])
+(form_goal
+“!A X a1:X ->A . isFun(a1) ==> !B a2:X->B.isFun(a2) ==>
+  !X0 x:X0->X.isFun(x) ==> Pa(a1,a2) o x = 
+Pa(a1 o x,a2 o x) ”));
+
+
+fun sspecl tl th = 
+    let val (b,vs) = strip_forall $ concl th
+        val ars = List.filter (fn (n,s) => not (on_ground o fst o dest_sort o snd $ (n,s))) vs
+        val env = match_tl essps (List.map mk_var ars) tl emptyvd
+        val tl' = List.map (inst_term env) (List.map mk_var vs)
+    in specl tl' th
+    end
+
+
+fun sspecl_then tl (ttac: thm_tactic): thm_tactic = 
+    fn th => ttac (aspecl tl th)
+
+val qsspecl_then = qterml_tcl aspecl_then
+
+val Pa_eq_eq = prove_store("Pa_eq_eq",
+e0
+(rpt strip_tac >> dimp_tac >> strip_tac >> arw[] >>
+ qby_tac ‘pi1(A,B) o Pa(f1, g1) = pi1(A,B) o Pa(f2, g2) &
+          pi2(A,B) o Pa(f1, g1) = pi2(A,B) o Pa(f2, g2)’
+ >-- arw[] >>
+ qsspecl_then [‘f1’,‘g1’] assume_tac pi12_of_Pa >> 
+ qsspecl_then [‘f2’,‘g2’] assume_tac pi12_of_Pa >> 
+ rfs[])
+(form_goal
+ “!A X f1:X->A.isFun(f1) ==> !f2:X->A.isFun(f2) ==>
+  !B g1:X->B. isFun(g1) ==> !g2:X->B. isFun(g2) ==> 
+  (Pa(f1,g1) = Pa(f2,g2) <=> f1 = f2 & g1 = g2)”));
+
+
+
+val Pa_eq_eq' = prove_store("Pa_eq_eq'",
+e0
+(rpt strip_tac >> irule Pa_eq_eq >> arw[])
+(form_goal
+ “!A X f1:X->A f2 B g1:X->B g2.isFun(f1) & isFun(f2) & isFun(g1) & isFun(g2) ==> 
+  (Pa(f1,g1) = Pa(f2,g2) <=> f1 = f2 & g1 = g2)”));
+
+
+val Thm1_case1_comm_condition_left = prove_store(
+"Thm1_case1_comm_condition_left",
+e0
+(rpt strip_tac >> qspecl_then [‘N’] assume_tac id_Fun >>
+ drule Pa_distr >> first_x_assum rev_drule >>
+ qspecl_then [‘N’,‘O’] assume_tac El_Fun >>
+ first_x_assum drule >> arw[idL] >>
+ dimp_tac >> strip_tac (* 2 *)
+ >-- (drule Pa_eq_eq >> 
+     qby_tac ‘isFun(f o El(O))’ 
+     >-- (irule o_Fun >> arw[El_Fun]) >>
+     first_x_assum drule >> 
+     first_x_assum drule >> first_x_assum rev_drule >>
+     fs[]) >>
+ arw[])
+(form_goal
+ “!B f:N->B. isFun(f) ==> !g:1->B. isFun(g) ==>
+ (Pa(id(N),f) o El(O) = Pa(El(O),g) <=> f o El(O) = g)”));
+
+
+val Thm1_case1_comm_condition_right = prove_store(
+"Thm1_case1_comm_condition_right",
+e0
+(rpt strip_tac >> 
+ qsspecl_then [‘SUC o pi1(N,B)’,‘h’,‘Pa(id(N),f)’] assume_tac Pa_distr'>>
+ qsspecl_then [‘id(N)’,‘f’,‘SUC’] assume_tac Pa_distr' >>
+ rfs[] >> 
+ assume_tac SUC_Fun >> 
+ qspecl_then [‘N’] assume_tac id_Fun >>
+ qspecl_then [‘N’,‘B’] assume_tac pi1_Fun >>
+ qsspecl_then [‘id(N)’,‘f’] assume_tac Pa_Fun >>
+ qsspecl_then [‘pi1(N,B)’,‘SUC’] assume_tac o_Fun >>
+ fs[] >> rfs[] >> fs[] >> rw[o_assoc,idL,idR] >>
+ qsspecl_then [‘id(N)’,‘f’] assume_tac pi1_of_Pa >> rfs[] >>
+ rw[idR] >>
+ qsspecl_then [‘SUC’,‘SUC’,‘h o Pa(id(N),f)’,‘f o SUC’] assume_tac Pa_eq_eq' >> 
+ qsspecl_then [‘SUC’,‘f’] assume_tac o_Fun >>
+ qsspecl_then [‘Pa(id(N),f)’,‘h’] assume_tac o_Fun >>
+ fs[] >> rfs[] >> fs[])
+(form_goal
+ “!B f:N->B. isFun(f) ==> !h:N * B ->B.isFun(h) ==>
+ (Pa(SUC o pi1(N,B),h) o Pa(id(N),f) = Pa(id(N),f) o SUC <=>
+ h o Pa(id(N),f) = f o SUC)”));
+
+val Thm1_case1_comm_condition = prove_store(
+"Thm1_case1_comm_condition",
+e0
+(rpt strip_tac >>  
+ drule Thm1_case1_comm_condition_left >> first_x_assum drule >>
+ drule Thm1_case1_comm_condition_right >> first_x_assum drule >>
+ arw[] >> dimp_tac >> strip_tac >> arw[])
+(form_goal
+ “!B f0:N->B g:1->B h:N * B -> B.
+  isFun(f0) & isFun(g) & isFun(h) ==> (f0 o El(O) = g & f0 o SUC = h o Pa(id(N),f0) <=>
+ Pa(id(N),f0) o El(O) = Pa(El(O),g) &
+ Pa(SUC o pi1(N,B),h) o Pa(id(N),f0) = Pa(id(N),f0) o SUC)”));
+
+
+
+val Dot_ex = prove_store("Dot_ex",
+e0
+(rpt strip_tac >> fs[Fun_expand] >>
+ first_x_assum (qspecl_then [‘dot’] strip_assume_tac) >>
+ last_x_assum (qspecl_then [‘dot’] strip_assume_tac) >>
+ rw[dot_def] >> qexists_tac ‘b’ >> arw[] >> rpt strip_tac >>
+ first_x_assum irule >> arw[])
+(form_goal
+ “!A f:1->A.isFun(f) ==> ?a. !d.Holds(f,d,a) &
+   (!a0 d. Holds(f,d,a0) ==> a0 = a)”)); 
+
+val Dot_def = Dot_ex |> spec_all |> ex2fsym "Dot" ["f"] 
+                     |> gen_all |> store_as "Dot_def";
+
+
+val Holds_El = prove_store("Holds_El",
+e0
+(rpt strip_tac >>  
+ qspecl_then [‘A’,‘a’] strip_assume_tac El_def >>
+ drule Eval_def >> arw[] >> flip_tac >> arw[dot_def])
+(form_goal
+ “!A a:mem(A) d. Holds(El(a),d,a)”));
+
+ 
+val Dot_of_El = prove_store("Dot_of_El",
+e0
+(rpt strip_tac >> qspecl_then [‘A’,‘a’] assume_tac El_Fun >> 
+ drule Dot_def >> first_x_assum (qspecl_then [‘dot’] strip_assume_tac) >>
+ flip_tac >> first_x_assum irule >> qexists_tac ‘dot’ >>
+ rw[Holds_El])
+(form_goal
+ “!A a:mem(A).Dot(El(a)) = a”));
 
 val Thm1_case_1 = prove_store("Thm1_case_1",
 e0
-(rpt strip_tac >> uex_tac >>
- assume_tac SUC_isFun >>
- qspecl_then [‘N’,‘B’] strip_assume_tac pi12_Fun >>
- qby_tac ‘isFun(SUC o pi1(N,B))’
- >-- (irule o_Fun >> arw[]) >>
- drule Nind_def
- assume_tac 
- abbrev_tac “Nind(Pair(O,g),Pa(SUC o pi1(N,B),h:N*B->B)) = f'” >>
- abbrev_tac “pi2(N,B) o f':N -> N * B = f” >>
- qby_tac ‘pi1(N,B) o f' = id(N)’
- >-- irule comm_with_SUC_id >> 
-     qpick_x_assum ‘Nind(Pair(O, g), Pa(SUC o pi1(N, B), h)) = f'’
-     (assume_tac o GSYM) >> arw[] >>
-     Nind_def
- qexists_tac ‘pi2(N,B) o Nind(Pair(O,g),Pa(SUC o pi1(N,B),h))’ >>
- )
+(rpt strip_tac >> uex_tac >> 
+ abbrev_tac “Nind(Pa(El(O),g:1->B),Pa(SUC o pi1(N,B),h:N * B->B)) = f'” >>
+ abbrev_tac “pi2(N,B) o f':N->N * B = f” >>
+ qby_tac ‘p1(N,B) o f' = id(N)’ >--
+ (irule comm_with_SUC_id >> 
+  qpick_x_assum ‘Nind(Pa(O, g), Pa(SUC o p1(N, B), h)) = f'’
+  (assume_tac o GSYM) >> arw[] >>
+  rw[o_assoc,Nind_def,p1_of_Pa] >> 
+  rw[GSYM o_assoc,p1_of_Pa]) >>
+ qby_tac ‘f' = Pa(id(N),f)’ >--
+ (once_rw[to_P_component] >> rw[p12_of_Pa] >> arw[]) >>
+ qexists_tac ‘f’ >>
+ qby_tac ‘f' o O = Pa(O,g) & 
+  f' o SUC = Pa(SUC o p1(N, B), h) o f'’ 
+ >-- (qpick_x_assum 
+     ‘Nind(Pa(O, g), Pa(SUC o p1(N, B), h)) = f'’
+     (assume_tac o GSYM) >> once_arw[] >>
+     rw[Nind_def]) >>
+ qby_tac ‘f o O = g & f o SUC = h o Pa(id(N), f)’
+ >-- (qpick_x_assum ‘p2(N, B) o f' = f’ (assume_tac o GSYM)>>
+      once_arw[] >> rw[o_assoc] >> once_arw[] >>
+      rw[GSYM o_assoc,p2_of_Pa] >>
+      pop_assum (K all_tac) >>
+      pop_assum (K all_tac) >> arw[]) >>
+ once_arw[] >> rw[] >>
+ rpt strip_tac >> 
+ qsuff_tac ‘Pa(id(N), f'') = Pa(id(N), f)’ 
+ >-- rw[Pa_eq_eq] >>
+ qsuff_tac ‘Pa(id(N), f'') = f'’ >-- arw[] >>
+ qsuff_tac ‘Pa(id(N), f'') = 
+  Nind(Pa(O, g), Pa(SUC o p1(N, B), h))’ >-- arw[] >>
+ irule is_Nind >> 
+ rw[Pa_distr,p1_of_Pa,o_assoc,idL,idR] >> once_arw[] >>
+ rw[])
 (form_goal
- “!B g:mem(B) h:N * B -> B. 
-  isFun(h) ==> ?!f:N->B. Eval(f,O) = g & f o SUC = h o Pa(id(N),f)”)));
+ “!B g:1->B h:N * B -> B. ?!f:N->B. f o El(O) = g & f o SUC = h o Pa(id(N),f)”));
+
+
+val is_Nind = Nind_El |> spec_all |> undisch |>spec_all |> conjE2
+                      |> conjE2 |> conjE2
+                      |> disch_all |> gen_all
+                      |> store_as "is_Nind";
+
+
+
+
+val o_eq_l = prove_store("o_eq_l",
+e0
+(rpt strip_tac >> arw[])
+(form_goal
+ “!B C g1:B->C g2:B->C. g1 = g2 ==>
+  !A f:A->B. g1 o f = g2 o f”));
+
+
+val o_eq_r = prove_store("o_eq_r",
+e0
+(rpt strip_tac >> arw[])
+(form_goal
+ “!A B f1:A->B f2:A->B. f1 = f2 ==>
+  !C g:B->C. g o f1 = g o f2”));
+
+
+
+
+val Pa_distr' = Pa_distr |> strip_all_and_imp |> conj_all_assum
+                         |> disch_all
+                         |> gen_all
+                         |> store_as "Pa_distr'"; 
+
+
+
+
+val pi1_Fun = pi12_Fun |> spec_all |> conjE1 |> gen_all
+                       |> store_as "pi1_Fun";
+
+
+
+val pi2_Fun = pi12_Fun |> spec_all |> conjE2 |> gen_all
+                       |> store_as "pi2_Fun";
+
+
+
+
+(*
+define the set of lists
+Eval(f:A(set of A->B functions)->B(set of A list -> B list function),a)
+
+induction recursion
+
+!P. P [] & (!t h.P(t) ==> P(h :: t)) ==> !l. P(l)
+
+recursion :
+
+!n c:'a -> 'b -> 'b. ?!f:'a list -> 'b. f [] = n & !h t. f(h :: t) = c h (f t)
+
+
+map fold
+
+
+Map(f:A->B): 'a list set -> 'b list set
+
+
+
+
+
+*)
+
+
+
+
+val ADD_def0 = Nind_def |> specl [rastt "N"]
+                        |> specl [rastt "SUC"]
+                        |> C mp SUC_Fun 
+                        
+
+
+(*
+pre0 
+pre0 n = (n,pre n)
+
+f: (n,pre n) |-> (suc n, n)
+
+
+(1, pre 1 = pre 0) |-> 
+*)
+
+
+val PRE_def0 = Nind_def |> specl [rastt "N * N"]
+                        |> specl [rastt "SUC"]
+                        |> C mp SUC_Fun 
+                        
